version with directed sets, theorem I complete

work.v
@@ -24,6 +24,41 @@ Definition Dbody_generalized X P (D:sig P) : X -> Prop :=
   proj1_sig D.
 *)
 
+(* First we define what are directed sets.
+    Here I do it completely naïvely, taking as argument the minimal needed. We could imagine also defining posets (or taking the def from the standard library), define directed sets over posets, and cpo as specific posets
+ *)
+Notation set X := (X -> Prop).
+Notation rel X := (X -> X -> Prop).
+Definition Directed {X} `(leq : rel X) (D : set X) : Prop :=
+  forall x y, D x -> D y -> exists z, D z /\ leq x z /\ leq y z.
+Definition directed_set {X} (leq : rel X) := {Dbody : set X | Directed leq Dbody}.
+Definition Dbody {X leq} (D : directed_set leq) : set X := proj1_sig D.
+
+(* Here we have the same fields as before, but we now call definitions that are not functions of CPO, but simply of operations that CPOs happen to have *)
+Class CPO (X: Type) := {
+  weq: relation X;
+  leq: relation X;
+  sup: directed_set leq -> X;
+  PreOrder_leq:> PreOrder leq;
+  weq_spec: forall x y, weq x y <-> (leq x y /\ leq y x);
+  sup_spec: forall D z, (leq (sup D) z <-> forall (y:X), (Dbody D) y -> leq y z);
+  }.
+
+Definition reverse_leq X (leq : X -> X -> Prop) : X -> X -> Prop := fun x y => leq y x.
+
+(* And now this work: notice that I pass `reverse_leq` to `Dbody` in the definition of `sup`.
+   If I am not mistaken that corresponds to what you were looking for, but I mostly followed the types without thinking of the semantics so I might be off :)
+ *)
+(*
+Global Program Instance reverse_CPO X (P: CPO X): CPO X := {|
+   weq := weq;
+   leq := reverse_leq leq;
+   sup D := sup (fun z => forall y, (@Dbody _ (reverse_leq leq) D y) -> leq z y);
+ |}.
+ *)
+ 
+(* Old versions *)
+(*
 Class CPO (X: Type) := {
   weq: relation X;
   leq: relation X;
@@ -36,7 +71,6 @@ Class CPO (X: Type) := {
   sup_spec: forall D z, (leq (sup D) z <-> forall (y:X), (Dbody D) y -> leq y z);
                         }.
 
-(*
 Class CPO (X: Type) := {
   weq: relation X;
   leq: relation X;
@@ -61,6 +95,8 @@ Global Hint Extern 0 => reflexivity: core.
 
 (** * Reversing a CPO *)
 
+(*Bad Idea, don't actually do it... *)
+(*
 Definition reverse_leq X (leq : X -> X -> Prop) : X -> X -> Prop := fun x y => leq y x.
 
 Global Program Instance reverse_CPO (P: CPO X): CPO X := {|
@@ -69,7 +105,8 @@ Global Program Instance reverse_CPO (P: CPO X): CPO X := {|
    sup D := sup (fun z => forall y, (@Dbody X (reverse_CPO X) D y) -> leq z y); 
    (*Careful ! I dunno which "leq" is used here :/*)
  |}.
-
+ Next Obligation.
+*)
 
 (** * Utilities  *)
 
@@ -85,23 +122,23 @@ Proof.
   apply weq_spec. split; apply Hf; (apply E || apply E').
 Qed.
 
-(** * General properties of complete lattices *)
+(** * General properties*)
 
 Section sup.
  Context {X} {P Q: CPO X} `{L : CompleteLattice X}.
  
  (*Below lemma is necessary for later property.*)
- Lemma directed_symmetry f g : (forall z, f z <-> g z) -> Directed f <-> Directed g.
+ Lemma directed_symmetry f g : (forall z, f z <-> g z) -> Directed leq f <-> Directed leq g.
  Proof.
   intro H. unfold Directed. (* unfold Directed_generalized. *)setoid_rewrite H. tauto.
 Qed.
 
 Definition iff_part (f g : X -> Prop) := forall z, f z <-> g z.
 Locate "<->".
-Global Instance directed_eq : Proper (iff_part ==> iff) Directed.
+Global Instance directed_eq : Proper (iff_part ==> iff) (Directed leq).
 Proof. intros f g. apply directed_symmetry. Qed.
 
-Lemma singleton_is_directed x : Directed (fun z => z=x).
+Lemma singleton_is_directed x : Directed leq (fun z => z=x).
 Proof.
   unfold Directed. intros. exists x. repeat split. now rewrite H. now rewrite H0.
 Qed.
@@ -144,6 +181,13 @@ Qed.
  Lemma leq_xsup_lat (Y:X->Prop) y : Y y -> y <= sup_lat Y.
  Proof. intro H. now apply (sup_spec_lat Y). Qed.
 
+Lemma sup_is_independent_of_proof : forall D_dir D_dir2, iff_part (Dbody D_dir) (Dbody D_dir2)
+  -> sup D_dir == sup D_dir2.
+Proof. 
+  intros. apply weq_spec. split; apply sup_spec; intros; apply leq_xsup;
+  now apply H.
+Qed.
+
 (*
 Lemma sup_unicity D s1 s2: sup D s1 -> sup D s2 -> s1 == s2.
 Proof.
@@ -151,7 +195,7 @@ Proof.
   now apply (sup_spec D s2). now apply (sup_spec D s1).
 Qed.*)
 
-Program Definition empty : directed_set := exist _ (fun _ => False) _.
+Program Definition empty : (directed_set leq) := exist _ (fun _ => False) _.
 Next Obligation.
 unfold Directed. (* unfold Directed_generalized.*) intros. contradict H.
 Defined.
@@ -214,8 +258,10 @@ Two solutions :
 --> Then we can make a lemma stating that the inf is actually the sup of lower elements 
 if this set is downward directed. 
 Try solution 2) to not "uselessly" weight down the definition of CPO.*)
+(* --> actually, no need for an inf ! We will instead define properties stating that an element is a least
+elements or things like that for the proofs. *)
 
-
+(*
  Definition inf Y := sup (fun z => forall y, Y y -> z <= y).
  Lemma inf_spec: forall Y z, Directed (fun z => forall y, Y y -> z <= y) -> z <= inf Y <-> (forall y, Y y -> z <= y).
  Proof.
@@ -235,8 +281,11 @@ Try solution 2) to not "uselessly" weight down the definition of CPO.*)
  Proof. intro H. now apply inf_spec. Qed.
  Lemma leq_xinf_lat (D: X -> Prop) y: D y -> inf D <= y.
  Proof. intro H. now apply inf_spec_lat with D. Qed.
+ *)
  
  (** other properties of binary joins *)
+ (* Still cups, still not handy now*)
+ (*
  Lemma leq_xcup x y z: Directed (fun t => t=x \/ t=y) -> z <= x \/ z <= y -> z <= cup x y.
  Proof.
   intro D. Check cup_spec.
@@ -257,10 +306,11 @@ Try solution 2) to not "uselessly" weight down the definition of CPO.*)
  Proof. auto using leq_xcup. Qed.
   Lemma cup_r_lat x y: y <= cup x y.
  Proof. auto using leq_xcup_lat. Qed.
-
+*)
 
 (*Below is possible but not practical to write with directedness condition, 
 do it later if needed*)
+(*
  Lemma cupA_lat x y z: cup x (cup y z) == cup (cup x y) z.
  Proof.
    apply from_above.
@@ -281,6 +331,7 @@ do it later if needed*)
    intro. rewrite !cup_spec_lat. tauto.
  Qed.
 
+
  Lemma or_reduce : forall A, A \/ A <-> A.
  Proof. tauto. Qed.
  Lemma cupI x: cup x x == x. (*done more generally with CPOs*)
@@ -290,24 +341,31 @@ do it later if needed*)
    apply directed_symmetry with (fun z => z=x). (*intuition.*) now setoid_rewrite or_reduce.
    apply singleton_is_directed.
  Qed.
+*)
 
 (* --- Inclusion of sets and includion of sups --- *)
 
 Definition included (S T: X -> Prop) := forall x, S x -> T x.
 Infix "⊆" := included (at level 70).
 
-Lemma sup_preserves_inclusion S T : S ⊆ T -> Directed S -> Directed T -> sup S <= sup T.
+#[global] Instance Included_trans : Transitive included.
 Proof.
-  intros H Ds Dt. apply sup_spec. assumption. intros. apply leq_xsup. assumption.
+  intros Y1 Y2 Y3 H12 H13. intros x H. apply H13. now apply H12.
+Qed.
+
+Lemma sup_preserves_inclusion S T : (Dbody S) ⊆ (Dbody T) -> sup S <= sup T.
+Proof.
+  intro H. apply sup_spec. intros. apply leq_xsup.
   now apply H.
 Qed.
 
-Lemma sup_preserves_eq S T : Directed S -> Directed T -> (forall x, S x <-> T x) -> sup S == sup T.
+Lemma sup_preserves_eq S T : (forall x, (Dbody S) x <-> (Dbody T) x) -> sup S == sup T.
 Proof.
   intros. apply weq_spec. split; apply sup_preserves_inclusion; 
-  [intros x Hx | assumption | assumption | intros x Hx | assumption | assumption]; now apply H1.
+  [intros x Hx | intros x Hx]; now apply H.
 Qed.
 
+(*
 Lemma included_inf_is_greater S T : S ⊆ T 
   -> Directed (fun z : X => forall y : X, S y -> z <= y)
  -> Directed (fun z : X => forall y0 : X, T y0 -> z <= y0) 
@@ -321,11 +379,11 @@ Lemma inf_preserves_eq (S T : X -> Prop) : Directed (fun z : X => forall y : X, 
 Proof.
   intros. apply weq_spec. split; apply included_inf_is_greater; 
   [intros x Hx | assumption | assumption | intros x Hx | assumption | assumption]; now apply H1.
-Qed.
+Qed.*)
 
 End sup.
 Global Hint Resolve bot_spec: core.
-Global Hint Resolve cup_l cup_r: core.
+(*Global Hint Resolve cup_l cup_r: core.*)
 
 
 Section functions.
@@ -333,7 +391,7 @@ Section functions.
  
  Record mon := { body:> X -> X; Hbody: Proper (leq ==> leq) body }.
  
- Global Instance Hbody' (F:mon) : Proper (weq ==> weq) F.
+ #[global] Instance Hbody' (F:mon) : Proper (weq ==> weq) F.
  Proof.
   apply (op_leq_weq_1 (Hf:=(Hbody F))).
 Qed.
@@ -342,21 +400,59 @@ Qed.
 Inductive Image f (S : X -> Prop) : X -> Prop :=
   |from_image : forall x, S x -> Image f S (f x).
 
-Definition Continuous φ := forall D, Directed D -> Directed (Image φ D)
-   /\ φ (sup D) = sup (Image φ D).
+Definition Image' f (S : set X) (y:X) := exists x, S x /\ y = f x.
 
-Definition Increasing F := forall x, x <= F x.
-
-Lemma mon_preserves_directedness_and_sup (F:mon) D : Directed D -> Directed (Image F D) /\ sup (Image F D) <= F (sup D).
-Proof. intros.
-  assert (Directed (Image F D)).
-  + unfold Directed. intros. inversion H0. inversion H1.
-  destruct (H x0 x1); try assumption. exists (F x2).
-  repeat split; try apply Hbody; apply H6.
-  + split. assumption. apply sup_spec. assumption. intros.
-    inversion H1. apply Hbody. now apply leq_xsup.
+Lemma im_eq : forall f S, iff_part (Image f S) (Image' f S).
+Proof.
+  intros f S x. split.
+  + intro. inversion H. now exists x0.
+  + intro. inversion H. destruct H0. rewrite H1. now apply from_image.
 Qed.
 
+Definition Continuous f := forall (D : set X) (H : Directed leq D), {dir_im : Directed leq (Image f D) & 
+  f (sup (exist _ D H )) == sup (exist _ (Image f D) dir_im)}. (*yup, dependent pair...*)
+
+(* Attempts at not making a dependent pair. Spoiler : it failed.*)
+(*
+Definition Continuous_im φ := forall (D: set X) (H:Directed leq D), Directed leq (Image φ D).
+
+Definition Continuous_1 φ := forall (D: set X) (H: Directed leq D), Directed leq (Image φ D).
+Definition Continuous φ := forall (D: set X) (H: Directed leq D), φ (sup (exist _ D H)) = sup (exist _ (Image φ D) (Continuous_1 φ D H)).
+
+Definition Image_dir φ S : (directed_set leq ):= exist _ (fun y => (exists x, y = φ x /\ ((Dbody S) x))) (Continuous_im φ).
+|from_image_dir : Continuous_im φ -> forall x, S x -> Image_dir φ S (φ x).
+
+Definition Continuous φ := forall (D: set X) (H:Directed leq D), Continuous_im φ /\ 
+  φ (sup (exist _ D H)) = sup (exist _ (Image φ D) (Continuous_im φ D H)).
+Next Obligation.
+  
+   /\ forall (D_dir:directed_set leq), φ (sup D_dir) = sup (exist (Directed leq) (Image φ (Dbody D_dir)) _).
+*)
+
+Lemma mon_preserves_directedness_and_sup (F:mon) : forall (D : set X) (H : Directed leq D), {dir_im : Directed leq (Image F D) & 
+  sup (exist _ (Image F D) dir_im) <= F (sup (exist _ D H ))}.
+Proof.
+  intros. assert (Directed leq (Image F D)). 
+  + unfold Directed. intros. inversion H0. inversion H1.
+    destruct (H x0 x1); try assumption. exists (F x2).
+    repeat split; try apply Hbody; apply H6.
+  + exists H0. apply sup_spec; cbn. intros.
+    inversion H1. apply Hbody. now apply leq_xsup.
+ Qed.
+
+(*same but with Image' to compare which definition is best in the proofs. And it seems to be less practical.*)
+Lemma mon_preserves_directedness_and_sup' (F:mon) : forall (D : set X) (H : Directed leq D), {dir_im : Directed leq (Image' F D) & 
+  sup (exist _ (Image' F D) dir_im) <= F (sup (exist _ D H ))}.
+Proof.
+  intros. assert (Directed leq (Image' F D)). 
+  + unfold Directed. intros. inversion H0. inversion H1.
+    destruct (H x0 x1); intuition. exists (F x2).
+    repeat split. now exists x2. rewrite H6. now apply Hbody.
+    rewrite H7. now apply Hbody.
+  + exists H0. apply sup_spec; cbn. intros.
+    inversion H1. destruct H2. rewrite H3. apply Hbody. now apply leq_xsup.
+ Qed.
+ 
 
 End functions.
 
@@ -364,13 +460,13 @@ End functions.
 
 
 
-(* Going on to Knaster-Tarski Theorem *)
+(* Knaster-Tarski Theorem on Lattices *)
 
 Section lattice_results.
 Context {X} `{L: CompleteLattice X}.
  Variable b: mon.
 
- Definition gfp := sup (fun x => x <= b x).
+ Definition gfp := sup_lat (fun x => x <= b x).
 
  Proposition leq_gfp: forall y, y <= b y -> y <= gfp.
  Proof. apply leq_xsup_lat. Qed.
@@ -406,10 +502,18 @@ Section fixpoint.
  Lemma fix_is_pre F : forall x, Fix F x -> Pre F x.
  Proof. intros. apply weq_spec in H. apply H. Qed.
  
+ (* Obsolete : we can't really define mu, it doesn't even always exists.
+ However, we can define a property stating that we are the least element of a set*)
+
+Definition is_least S x := S x /\ forall y, S y -> x <= y.
+Definition is_inf S x := forall z, (forall y, S y -> z <= y) <-> z <= x.
+ 
+ (*
  Notation µ F := (inf (fun x => Fix F x)). (*Rmq : Attention, on préférerait que ce soit un min.
  Cependant, s'il existe, il est égal à l'inf donc c'est bon.*)
  
  Definition mu_exists F := Directed (fun z => forall y, (fun x => Fix F x) y -> z <= y) /\ Fix F (µ F).
+ *)
  
  Fixpoint itere F n x0 : X := match n with
   | 0 => x0
@@ -487,7 +591,7 @@ Lemma comparison : forall (n m:nat), le n m \/ le m n.
 Proof. intros n m. case_eq
 *)
 
-Lemma iteres_directed (F:mon): Directed (iteres F).
+Lemma iteres_directed (F:mon): Directed leq (iteres F).
 Proof.
   unfold Directed. intros. destruct H. destruct H0.
   case_eq (Nat.compare n n0); intro H.
@@ -502,28 +606,20 @@ Proof.
   + exists (itere F n bot). repeat split. reflexivity. now apply chain_increase.
 Qed.
 
+(*
+Program Definition iteres_dir (F:mon) := (exist _ (iteres F) (iteres_directed F)).*)
+(*Program Definition α (F:mon) := (sup (exist _ (iteres F) _)).
+Next Obligation. apply (iteres_directed F). Qed.*)
+(* Notation α F := (sup (iteres F)).*)
+Definition α (F:mon) := (sup (exist (Directed leq) (iteres F) (iteres_directed F))).
 
-
- Notation α F := (sup (iteres F)).
-
- Theorem Fixpoint_I_i (F:mon) : Fix F (α F) -> mu_exists F /\ α F == µ F.
+ Theorem Fixpoint_I_i (F:mon) : Fix F (α F) -> is_least (Fix F) (α F).
  Proof.
- intro H. 
- assert (forall β, Fix F β -> α F <= β). (*alpha is the least fixpoint.*)
-  intros. apply sup_spec. apply iteres_directed. intros y Q.
-  inversion Q. rewrite <- (itere_preserves_fix F β n).
+ intro H. split; try assumption.
+  intros. apply sup_spec; cbn. intros z Q.
+  inversion Q. rewrite <- (itere_preserves_fix F y n).
   now apply itere_monotony. assumption.
- assert (Directed (fun z : X => forall y : X, Fix F y -> z <= y)). (*mu is well defined*)
-    unfold Directed. intros. exists (α F). repeat split. intros. now apply H0.
-    now apply H1. now apply H2.
-  assert (α F == µ F). apply weq_spec. split.
-   - apply inf_spec. apply H1. assumption.
-   - apply leq_xinf. apply H1. assumption.
-   - unfold mu_exists. repeat split. assumption.
-    unfold Fix. rewrite <- H2. apply H. assumption.
 Qed.
-
-
 
 
 (* ---------------------- Theorem I (ii) ---------------------------------- *)
@@ -531,7 +627,7 @@ Qed.
 Inductive iteres_from_1 F : X -> Prop := 
   | from_bot_from_1 : forall n,  le 1 n -> iteres_from_1 F (itere F n bot).
   
-Lemma iteres_from_1_directed (F:mon): Directed (iteres_from_1 F).
+Lemma iteres_from_1_directed (F:mon): Directed leq (iteres_from_1 F).
 Proof.
   unfold Directed. intros. destruct H. destruct H0.
   destruct le_ge_dec with n n0.
@@ -540,7 +636,7 @@ Proof.
 Qed.
 
 Lemma image_of_iteres F : forall x, (Image F (iteres F)) x <-> (iteres_from_1 F) x.
-Proof.
+Proof. (*TODO : rewrite this with iff_part ? And add a reserved notation for iff_part.*)
   intro. split; intro; inversion H. inversion H0.
   + assert (iteres_from_1 F (itere F (S n) bot)). apply from_bot_from_1. lia.
     apply H3.
@@ -553,62 +649,54 @@ Proof.
   intros x H. inversion H. apply from_bot.
 Qed.
 
-Lemma sup_from_1 (F:mon) : α F == sup (iteres_from_1 F).
+Program Definition α' (F:mon) := (sup (exist _ (iteres_from_1 F) _)).
+Next Obligation. apply iteres_from_1_directed. Qed.
+
+Lemma sup_from_1 (F:mon) : α F == α' F.
 Proof.
   apply weq_spec. split. 
-  + apply sup_spec. apply iteres_directed. intros. inversion H.
-  induction n. now cbn.
-  apply leq_xsup. apply iteres_from_1_directed.
+  + apply sup_spec; cbn. intros. inversion H.
+  induction n. now cbn. apply leq_xsup.
   apply from_bot_from_1. lia.
-  + apply sup_preserves_inclusion. apply from_1_included.
-  apply iteres_from_1_directed. apply iteres_directed.
+  + apply sup_preserves_inclusion; cbn. apply from_1_included.
 Qed.
 
 (* Fix F (mu F) is here to say that "mu F exists", cause it is supposed to be a min and not an inf. *)
-Theorem Fixpoint_I_ii (F:mon) : Continuous F -> mu_exists F /\ α F == µ F.
+Theorem Fixpoint_I_ii (F:mon) : Continuous F -> is_least (Fix F) (α F).
 Proof.
-  intro H. assert (Fix F (α F)).
-  + unfold Fix. destruct H with (iteres F). apply iteres_directed. rewrite H1.
-  transitivity (sup (iteres_from_1 F)). apply sup_preserves_eq. assumption. 
-  apply iteres_from_1_directed. apply image_of_iteres. now rewrite sup_from_1.
-  + now apply Fixpoint_I_i.
+  intro H.
+  assert (Fix F (α F)).
+   + unfold Fix. destruct (H (iteres F) (iteres_directed F)) as [HD HS].
+    transitivity (α' F); try now rewrite sup_from_1. rewrite HS.
+    apply sup_is_independent_of_proof. cbn. unfold iff_part. apply image_of_iteres.
+   + now apply Fixpoint_I_i.
 Qed.
 
 
 
 (* ------------------------- Theorem II ------------------------------ *)
 
+(*
 Notation µ0 F := (inf (fun x => Pre F x)). 
-
- Definition mu0_exists F := Directed (fun z => forall y, (fun x => Pre F x) y -> z <= y) /\ Pre F (µ0 F).
+ Definition mu0_exists F := Directed (fun z => forall y, (fun x => Pre F x) y -> z <= y) /\ Pre F (µ0 F).*)
 (*Warning : this is delicate. "If the least prefixpoint exists, we write it mu0" is not easily written in Coq.
 I could also replace mu0_exists (and mu_exists) with the properties of a least prefixpoint, but to prove it from
 the def of the inf I would still need the inf to be well defined, ie. this set to be directed.
 I think it could be possible for this set to NOT be directed (so inf not well defined), but for such a least prefixpoint
 to still exist. In that case I will not know how to define it at all. It will just be a "exists" proposition.*)
 
-Lemma Induction_Rule (F:mon) : mu0_exists F -> mu_exists F /\ forall x, Pre F x -> µ F <= x.
-Proof.
-  intro H. destruct H.
-  assert (Fix F (µ0 F)).
-    apply weq_spec. split. apply H0.
-    apply leq_xinf. assumption. unfold Pre. apply Hbody. apply H0.
-  
-  assert (Directed (fun z : X => forall y : X, Fix F y -> z <= y)).
-    unfold Directed. intros. exists (µ0 F). repeat split. intros.
-    apply leq_xinf. assumption. now apply fix_is_pre.
-    now apply H2. now apply H3.
-  
-  assert (µ F == µ0 F).
-    apply weq_spec. split. apply leq_xinf; assumption.
-    apply included_inf_is_greater; try assumption. intros x Hx. now apply fix_is_pre.
-  
-  repeat split.
-  + assumption.
-  + unfold Fix. rewrite H3. apply H1.
-  + intros. rewrite H3. apply leq_xinf; assumption.
-Qed.
+(* --> is_least (Pre F) x already means what I want.*)
 
+Lemma Induction_Rule (F:mon) : (exists µ0, is_least (Pre F) µ0)
+  -> exists µ, is_least (Fix F) µ /\ forall x, Pre F x -> µ <= x.
+Proof.
+  intro H. destruct H as [µ0 Hmu0].
+  exists µ0. repeat split.
+  + apply weq_spec. split. apply Hmu0.
+    apply Hmu0. unfold Pre. apply Hbody. apply Hmu0.
+  + intros. apply Hmu0. now apply fix_is_pre.
+  + apply Hmu0.
+Qed.
 
 
 
@@ -635,106 +723,174 @@ Program Definition const x: mon := {| body y := x |}.
  
 
 
-Global Program Instance CPO_mon: CPO mon := {|
+Program Instance CPO_mon: CPO mon := {|
    weq := pointwise_relation X weq;
    leq := pointwise_relation X leq;
    sup F := {| body a := sup (fun b => exists2 f, F f & b=f a) |};
  |}.
- Next Obligation.
-   intros x y H. apply sup_spec.
-   unfold Directed. intros. destruct H0 as [f1 Ff1 f1x0]. destruct H1 as [f2 Ff2 f2y0].
-   exists (f2 x). repeat split. now exists f2.
-   
-   intros i [f Ff ->].
-   rewrite H. apply leq_xsup. eauto. 
- Qed.
- Next Obligation. constructor. now intros f x. intros f g h H H' x. now transitivity (g x). Qed.
- Next Obligation. unfold pointwise_relation. setoid_rewrite weq_spec. firstorder. Qed.
- Next Obligation.
-   unfold pointwise_relation. setoid_rewrite sup_spec.
-   firstorder. rewrite H1. auto. 
- Qed.
-
-
- Record mon_inc := { Ibody:> X -> X; HMbody: Proper (leq ==> leq) Ibody; HIbody : Increasing Ibody}.
- 
- Instance HIbody' (f: mon_inc): Proper (weq ==> weq) f.
- Proof. intros x y. rewrite 2weq_spec. now split; apply f. Qed.
-
- (** constant function *)
- Program Definition const x: mon_inc := {| Ibody y := x |}.
- Next Obligation. intros ? ? ?. reflexivity. Qed.
-
- (** identity and composition
-     the monotonicity proofs are transparent to get strong equalities
-     - [id ° f = f ° id = f], and
-     - [f ° (g ° h) = (f ° g) ° h]
-  *)
- Definition id: mon_inc := {| 
-   Ibody x := x; 
-   HMbody x y H := H;
-   HIbody x := (reflexivity x)
- |}.
-
-(*
- Definition comp (f g: mon_inc): mon_inc := {|
-   body := fun x => f (g x); 
-   Hbody x y H := Hbody f _ _ (Hbody g _ _ H) 
- |}.
- Infix "°" := comp (at level 20): lattice.
- *)
- 
- (** monotone increasing endofunctions form a new CPO *)
- Global Program Instance CPO_increasing_mon: CPO mon_inc := {|
-   weq := pointwise_relation X weq;
-   leq := pointwise_relation X leq;
-   sup F := {| Ibody a := sup (fun b => exists2 f, F f & b=f a) |};
- |}.
- Next Obligation.
-   intros x y H. apply sup_spec. intros i [f Ff ->].
-   rewrite H. apply leq_xsup. eauto. 
- Qed.
- Next Obligation. constructor. now intros f x. intros f g h H H' x. now transitivity (g x). Qed.
- Next Obligation. unfold pointwise_relation. setoid_rewrite weq_spec. firstorder. Qed.
- Next Obligation.
-   unfold pointwise_relation. setoid_rewrite sup_spec.
-   firstorder. rewrite H1. auto. 
- Qed.
-
-
-
-
-
-
-
-Program Instance CPO_self_maps_mon :  CPO (X -> X) :=
-  {| weq:=pointwise_relation X weq;
-     leq:=pointwise_relation X leq;
-     sup F a:=sup (fun b => exists2 f, F f & b=f a);
-  |}.
-Next Obligation. 
-  constructor.
-   now intros f x. 
-   intros f g h H H' x. now transitivity (g x).
-Qed.
-Next Obligation. unfold pointwise_relation. setoid_rewrite weq_spec. firstorder. Qed.
 Next Obligation.
-  unfold pointwise_relation. setoid_rewrite sup_spec.
-  firstorder. rewrite H1. now apply H. 
+  unfold Directed. intros. destruct F as [SF D]; cbn in *.
+  destruct H as [fx Hfx]. destruct H0 as [fy Hfy].
+  destruct (D fx fy) as [f [Hf1S [Hff1 Hff2]]]; try assumption.
+  exists (f a). repeat split. now exists f.
+  + rewrite H. apply Hff1.
+  + rewrite H0. apply Hff2.
 Qed.
-(*below : a simpler version of lemma 8.21 used in theorem. Only need existence of a FixPoint.*)
-Lemma increasing_has_fix_point (F:mon) : Increasing F -> Fix F (α F).
+Next Obligation.
+  destruct F as [SF D]; cbn in *.
+  intros x y H. apply sup_spec; cbn. intros.
+  destruct H0 as [f Hf].
+  transitivity (f y). rewrite H0. now apply Hbody.
+  apply leq_xsup. cbn. now exists f.
+Qed.
+Next Obligation. (*Rmk : symbol ":>" is to declare a trivial instance.*)
+  apply Build_PreOrder.
+  + intro x. reflexivity.
+  + intros f g h Hfg Hgh x. now transitivity (g x).
+Qed.
+Next Obligation.
+  split; intros.
+  + split; intro a; now apply weq_spec.
+  + intro. now apply weq_spec.
+Qed.
+Next Obligation.
+  destruct D as [SF D]; cbn in *. split. 
+  + intros H f Df x. rewrite <- (H x).
+  apply (sup_spec (exist (fun Dbody0 : set X => Directed leq Dbody0)
+     (fun b : X => exists2 f0 : mon, SF f0 & b = f0 x)
+     (CPO_mon_obligation_1
+        (exist
+           (fun Dbody0 : set mon =>
+            Directed (fun x0 x1 : mon => pointwise_relation X leq x0 x1)
+              Dbody0) SF D) x))).
+  reflexivity.
+  cbn. now exists f.
+  + intros H x. apply sup_spec. intros. inversion H0. rewrite H2. now apply (H x0).
+Qed.
+
+Program Instance CPO_parts: CPO (set X) := {|
+   weq := iff_part;
+   leq := included;
+   sup A := (fun x => exists Y, A Y /\ Y x);
+ |}.
+Next Obligation.
+  apply Build_PreOrder.
+  + intro Y. now intro x.
+  + apply Included_trans.
+Qed.
+Next Obligation.
+  repeat split; try intuition; intros a; intro H0; apply H; try apply H0.
+Qed.
+Next Obligation.
+  split; intros; intros a Ha. apply H. now exists y.
+  destruct Ha. apply (H x). apply H0. apply H0.
+Qed.
+
+Program Instance Lattice_parts : CompleteLattice (CPO_parts) := {|
+  sup_lat A := (fun x => exists Y, A Y /\ Y x); 
+ |}.
+Next Obligation.
+  split; intros; intros a Ha. apply H. now exists y.
+  destruct Ha. apply (H x). apply H0. apply H0.
+Qed.
+
+
+Definition Increasing (F:@mon X P) := forall (x:X), x <= F x.
+Check Increasing.
+
+(*Program Definition I := exist _ Increasing _.*)
+
+Program Definition I := exist (Directed (@leq mon CPO_mon)) (Increasing (*:set (@mon X P)*)) _. 
+Next Obligation.
+  (*unfold I_obligation_1.*)
+  unfold Directed. intros f g Hf Hg. exists (comp f g). repeat split.
+  + intro x. transitivity (g x). apply Hg. apply Hf.
+  + intro x. cbn. apply Hbody. apply Hg.
+  + intro x. cbn. apply Hf.
+Defined.
+
+Notation H_sup := (sup I).
+
+Lemma H_sup_is_increasing : Increasing H_sup.
 Proof.
-  intro. unfold Fix. apply weq_spec. unfold Increasing in H. split.
-  + Check sup_spec. apply sup_spec with (iteres F). apply iteres_directed. reflexivity. .
+  intro. assert (id <= H_sup). now apply (sup_spec I). apply H. Qed.
+
+(*below : a simpler version of lemma 8.21 used in theorem. Only need existence of a FixPoint,
+not of a common Fixpoint for all Increasing function.*)
+Lemma increasing_has_fix_point (F:@mon X P) : Increasing F -> exists x, Fix F x.
+Proof.
+  intro. exists (H_sup bot).
+  assert ((comp F H_sup) == H_sup).
+  + apply weq_spec. split. apply (sup_spec I). reflexivity. 
+    intro. transitivity (H_sup x). apply H_sup_is_increasing. apply H.
+    intro. apply H.
+  + unfold Fix. now setoid_rewrite (H0 bot).
 Qed.
+
+Definition Invariant F (Y: set X) := included Y (Image F Y).
+
+Definition P0 (F:@mon X P) := (fun x => forall Y, Invariant F Y -> Y x). 
+(* intersection of all invariant sub-CPOs *)
+
+Program Definition Φ (F:@mon X P) : @mon (set X) (CPO_parts) :=  (*since def of mon is linked to that of CPOs, need a CPO of parts*)
+  {| body X := (fun x => (x = bot \/ (Image F X) x \/ (exists D, included (Dbody D) X /\ x = sup D))) |}.
+Next Obligation.
+  intros Y1 Y2 H12 x Hx. destruct Hx; intuition. 
+  + right. left. inversion H0. apply from_image. now apply H12.
+  + destruct H0 as [Hd [Hi Hs]]. right. right. exists Hd. split.
+    intros y Hy. apply H12. now apply Hi. assumption.
+Qed.
+
+Definition P0' F := gfp (Φ F). (* sup_lat (fun x => x <= Φ F x).*)
+Check P0.
+Check P0'.
+
+Lemma P0_is_P0' F : (P0 F) == (P0' F).
+Proof. (*dunno why this is true;*)
+  apply weq_spec. split.
+  Print leq_gfp.
+   apply leq_xsup_lat. intros x H.
+  apply H. intros y Hy. cbn. Search "Image". apply im_eq. Print Image'. destruct Hy. rewrite H0. cbn.
+  
+  apply (sup_spec_lat (fun x => x <= Φ F x)). intros x H.
+
+Lemma P0_is_in_Post (F:@mon X P) : included (P0 F) (Post F).
+Proof.
+  assert (Invariant F (Post F)).
+  + Check Induction_Rule.
+
+Theorem Fixpoint_II (F:@mon X P) : exists x, Fix F x.
+Proof.
+  
 
 End fixpoint.
 
 
 
 
+Section lattice_results.
+Context {X} `{L: CompleteLattice X}.
+ Variable b: mon.
 
+ Definition gfp := sup_lat (fun x => x <= b x).
+
+ Proposition leq_gfp: forall y, y <= b y -> y <= gfp.
+ Proof. apply leq_xsup_lat. Qed.
+
+ Lemma gfp_pfp: gfp <= b gfp.
+Proof.
+  unfold gfp. apply sup_spec_lat. intros y H. rewrite H. apply Hbody.
+  apply leq_xsup_lat. apply H.
+Qed.
+
+ Lemma gfp_fp: gfp == b gfp.
+Proof.
+  rewrite weq_spec. split.
+    + apply gfp_pfp.
+    + apply leq_xsup_lat. apply Hbody. apply gfp_pfp.
+Qed.
+
+End lattice_results.
 
 
 
@@ -865,30 +1021,6 @@ Instance app_leq {X} {L: CompleteLattice X}: Proper (leq ==> leq ==> leq) body.
 Proof. intros f g fg x y xy. transitivity (f y). now apply f. now apply fg. Qed.
 Instance app_weq {X} {L: CompleteLattice X}: Proper (weq ==> weq ==> weq) body := op_leq_weq_2.
 
-
-(** * Knaster-Tarski *)
-Section s.
-    
- Context {X} {L: CompleteLattice X}.
- Variable b: mon X.
-
- Definition gfp := sup (fun x => x <= b x).
-
- Proposition leq_gfp: forall y, y <= b y -> y <= gfp.
- Proof. apply leq_xsup. Qed.
-
- Lemma gfp_pfp: gfp <= b gfp.
-Proof.
-  unfold gfp. apply sup_spec. intros y H. rewrite H. apply Hbody.
-  apply leq_xsup. apply H.
-Qed.
-
- Lemma gfp_fp: gfp == b gfp.
-Proof.
-  rewrite weq_spec. split.
-    + apply gfp_pfp.
-    + apply leq_xsup. apply Hbody. apply gfp_pfp.
-Qed.
 
 
 (** * Compatibility *)
